update CDDL.Spec from project-everest/everparse@659e2d75fd8740841c295bc27687d3b55480d8cb

share/pulse/examples/dice/cbor/CDDL.Spec.fsti
@@ -229,12 +229,41 @@ let rec list_is_suffix_of_precedes
     else list_is_suffix_of_precedes v0 small (List.Tot.tl large)
   end
 
+let opt_precedes_list_item
+  (#t1 #t2: Type)
+  (x2: option t2)
+  (x1: t1)
+: GTot bool
+= FStar.StrongExcludedMiddle.strong_excluded_middle (opt_precedes x1 x2)
+
+module Pull = FStar.Ghost.Pull
+
+noextract
+let opt_precedes_list
+  (#t1 #t2: Type)
+  (l: list t1)
+  (b: option t2)
+: Tot prop
+= List.Tot.for_all (Pull.pull (opt_precedes_list_item b)) l
+
+let rec opt_precedes_opt_precedes_list
+  (#t1 #t2: Type)
+  (l: list t1)
+  (b: option t2)
+: Lemma
+  (requires (opt_precedes l b))
+  (ensures (opt_precedes_list l b))
+  [SMTPat (opt_precedes_list l b)]
+= match l with
+  | [] -> ()
+  | a :: q -> opt_precedes_opt_precedes_list q b
+
 [@@erasable; noextract_to "krml"]
-let array_group3 (bound: option Cbor.raw_data_item) = (l: list Cbor.raw_data_item { opt_precedes l bound }) -> Ghost (option (list Cbor.raw_data_item))
+let array_group3 (bound: option Cbor.raw_data_item) = (l: list Cbor.raw_data_item { opt_precedes_list l bound }) -> Ghost (option (list Cbor.raw_data_item & list Cbor.raw_data_item))
   (requires True)
   (ensures (fun l' -> match l' with
   | None -> True
-  | Some l' -> opt_precedes l' bound
+  | Some (l1, l2) -> l == l1 `List.Tot.append` l2
   ))
 
 noextract
@@ -245,12 +274,25 @@ let array_group3_equiv
 = forall l . g1 l == g2 l
 
 let array_group3_always_false #b : array_group3 b = fun _ -> None
-let array_group3_empty #b : array_group3 b = fun x -> Some x
+
+let opt_precedes_list_assoc
+  (#t1 #t2: Type)
+  (l1 l2: list t1)
+  (b: option t2)
+: Lemma
+  (opt_precedes_list (l1 `List.Tot.append` l2) b <==>  opt_precedes_list l1 b /\ opt_precedes_list l2 b)
+  [SMTPat (opt_precedes_list (l1 `List.Tot.append` l2) b)]
+= List.Tot.for_all_append (Pull.pull (opt_precedes_list_item b)) l1 l2
+
+let array_group3_empty #b : array_group3 b = fun x -> Some ([], x)
 let array_group3_concat #b (a1 a3: array_group3 b) : array_group3 b =
   (fun l ->
     match a1 l with
     | None -> None
-    | Some l3 -> a3 l3
+    | Some (l1, l2) ->  begin match a3 l2 with
+      | None -> None
+      | Some (l3, l4) -> List.Tot.append_assoc l1 l3 l4; Some (List.Tot.append l1 l3, l4)
+    end
   )
 
 let array_group3_concat_equiv
@@ -261,24 +303,607 @@ let array_group3_concat_equiv
   (ensures ((a1 `array_group3_concat` a2) `array_group3_equiv` (a1' `array_group3_concat` a2')))
 = ()
 
+let array_group3_concat_unique_strong
+  #b (a1 a3: array_group3 b)
+: Tot prop
+= (forall (l: (l: list Cbor.raw_data_item { opt_precedes_list l b })) (l' rem: list Cbor.raw_data_item) .
+    array_group3_concat a1 a3 l == Some (l', rem) <==> (
+      (exists (l1 l2 l3: list Cbor.raw_data_item) .
+        l == l1 `List.Tot.append` l2 /\
+        a1 l1 == Some (l1, []) /\
+        a3 l2 == Some (l3, rem) /\
+        l' == l1 `List.Tot.append` l3
+  ))) /\
+  (forall (l1 l2: (l: list Cbor.raw_data_item { opt_precedes_list l b })) .
+    (a1 l1 == Some (l1, []) /\ Some? (a3 l2)) ==>
+    a1 (l1 `List.Tot.append` l2) == Some (l1, l2)
+  )
+
+let array_group3_concat_unique_strong_prop_intro
+  #b (a1 a3: array_group3 b)
+  (l1 l2: (l: list Cbor.raw_data_item { opt_precedes_list l b }))
+  (l3 rem: list Cbor.raw_data_item)
+: Lemma
+  (requires (
+    array_group3_concat_unique_strong a1 a3 /\
+    (a1 l1 == Some (l1, []) /\ a3 l2 == Some (l3, rem))
+  ))
+  (ensures (
+      array_group3_concat a1 a3 (l1 `List.Tot.append` l2) == Some (l1 `List.Tot.append` l3, rem)
+  ))
+= ()
+
+let array_group3_concat_unique_strong_prop_elim_gen
+  #b (a1 a3: array_group3 b)
+  (l: list Cbor.raw_data_item { opt_precedes_list l b })
+  (l' rem: list Cbor.raw_data_item)
+: Lemma
+  (requires (
+    array_group3_concat_unique_strong a1 a3 /\
+    array_group3_concat a1 a3 l == Some (l', rem)
+  ))
+  (ensures (
+      (exists (l1 l2 l3: list Cbor.raw_data_item) .
+        a1 l == Some (l1, l2) /\
+        a1 l1 == Some (l1, []) /\
+        a3 l2 == Some (l3, rem) /\
+        l' == l1 `List.Tot.append` l3
+  )))
+= ()
+
+let array_group3_concat_unique_strong_prop_elim
+  #b (a1 a3: array_group3 b)
+  (l: list Cbor.raw_data_item { opt_precedes_list l b })
+: Lemma
+  (requires (
+    array_group3_concat_unique_strong a1 a3 /\
+    array_group3_concat a1 a3 l == Some (l, [])
+  ))
+  (ensures (
+      (exists (l1 l2: list Cbor.raw_data_item) .
+        a1 l == Some (l1, l2) /\
+        a1 l1 == Some (l1, []) /\
+        a3 l2 == Some (l2, []))
+  ))
+= array_group3_concat_unique_strong_prop_elim_gen a1 a3 l l [];
+  let Some (l1, l2) = a1 l in
+  let Some (l3, _) = a3 l2 in
+  List.Tot.append_l_nil l3
+
+let array_group3_concat_unique_strong_intro
+  #b (a1 a3: array_group3 b)
+: Lemma
+  (requires (
+    forall (l1 l2: (l: list Cbor.raw_data_item { opt_precedes_list l b })) .
+      Some? (a3 l2) ==> (a1 l1 == Some (l1, []) <==> a1 (l1 `List.Tot.append` l2) == Some (l1, l2))
+  ))
+  (ensures (
+    array_group3_concat_unique_strong a1 a3
+  ))
+= ()
+
+let array_group3_concat_unique_strong_elim1
+  #b (a1 a3: array_group3 b)
+: Lemma
+  (requires (
+    array_group3_concat_unique_strong a1 a3
+  ))
+  (ensures (
+    forall (l1 l2: (l: list Cbor.raw_data_item { opt_precedes_list l b })) .
+      Some? (a3 l2) ==> (a1 l1 == Some (l1, []) ==> a1 (l1 `List.Tot.append` l2) == Some (l1, l2))
+  ))
+= ()
+
+let indefinite_description_ghost3
+  #t1 #t2 #t3
+  (p: t1 -> t2 -> t3 -> prop)
+: Ghost (t1 & t2 & t3)
+    (requires (exists x1 x2 x3 . p x1 x2 x3))
+    (ensures (fun (x1, x2, x3) -> p x1 x2 x3))
+= let x1 = FStar.IndefiniteDescription.indefinite_description_ghost t1 (fun x1 -> exists x2 x3 . p x1 x2 x3) in
+  let x2 = FStar.IndefiniteDescription.indefinite_description_ghost t2 (fun x2 -> exists x3 . p x1 x2 x3) in
+  let x3 = FStar.IndefiniteDescription.indefinite_description_ghost t3 (fun x3 -> p x1 x2 x3) in
+  (x1, x2, x3)
+
+let array_group3_concat_unique_strong_elim2
+  #b (a1 a3: array_group3 b)
+: Lemma
+  (requires (array_group3_concat_unique_strong a1 a3))
+  (ensures (
+    forall (l1 l2: (l: list Cbor.raw_data_item { opt_precedes_list l b })) .
+      Some? (a3 l2) ==> (a1 (l1 `List.Tot.append` l2) == Some (l1, l2) ==> a1 l1 == Some (l1, []))
+  ))
+= let prf
+      (l1 l2: (l: list Cbor.raw_data_item { opt_precedes_list l b }))
+  : Lemma
+    ((Some? (a3 l2) /\ a1 (l1 `List.Tot.append` l2) == Some (l1, l2)) ==> a1 l1 == Some (l1, []))
+  = if FStar.StrongExcludedMiddle.strong_excluded_middle (Some? (a3 l2) /\ a1 (l1 `List.Tot.append` l2) == Some ((l1 <: list _), (l2 <: list _)))
+    then begin
+      let Some (l3, rem) = a3 l2 in
+      let l' = l1 `List.Tot.append` l3 in
+      let l = l1 `List.Tot.append` l2 in
+      array_group3_concat_unique_strong_prop_elim_gen a1 a3 l l' rem
+    end
+  in
+  Classical.forall_intro_2 prf
+
+noextract
+let array_group3_concat_unique_strong'
+  #b (a1 a3: array_group3 b)
+: Tot prop
+=
+    forall (l1 l2: (l: list Cbor.raw_data_item { opt_precedes_list l b })) .
+      Some? (a3 l2) ==> (a1 (l1 `List.Tot.append` l2) == Some (l1, l2) <==> a1 l1 == Some (l1, []))
+
+let array_group3_concat_unique_strong_equiv
+  #b (a1 a3: array_group3 b)
+: Lemma
+  (array_group3_concat_unique_strong a1 a3 <==> array_group3_concat_unique_strong' a1 a3)
+  [SMTPat (array_group3_concat_unique_strong a1 a3)]
+= Classical.move_requires (array_group3_concat_unique_strong_elim2 a1) a3
+
+let array_group3_strong_prefix
+  #b (a1: array_group3 b)
+: Tot prop
+= forall (l1 l2: (l: list Cbor.raw_data_item { opt_precedes_list l b })) .
+    (a1 l1 == Some (l1, []) <==> a1 (l1 `List.Tot.append` l2) == Some (l1, l2))
+
+let array_group3_strong_prefix_empty
+  (b: option Cbor.raw_data_item)
+: Lemma
+  (array_group3_strong_prefix #b array_group3_empty)
+= ()
+
+let array_group3_strong_prefix_implies_concat_unique_strong
+  #b (a1 a3: array_group3 b)
+: Lemma
+  (array_group3_strong_prefix a1 ==> array_group3_concat_unique_strong a1 a3)
+= ()
+
+let array_group3_concat_unique_strong'_strong_prefix
+  #b (a1 a2: array_group3 b)
+: Lemma
+  (requires (
+    array_group3_concat_unique_strong' a1 a2 /\
+    array_group3_strong_prefix a2
+  ))
+  (ensures (
+    array_group3_strong_prefix (array_group3_concat a1 a2)
+  ))
+= let a = array_group3_concat a1 a2 in
+  let prf
+    (l1 l2: (l: list Cbor.raw_data_item { opt_precedes_list l b }))
+  : Lemma
+    (a l1 == Some (l1, []) ==> a (l1 `List.Tot.append` l2) == Some (l1, l2))
+  = if FStar.StrongExcludedMiddle.strong_excluded_middle (a l1 == Some (l1, []))
+    then begin
+      let Some (l11, l12) = a1 l1 in
+      List.Tot.append_assoc l11 l12 l2
+    end
+    else ()
+  in
+  Classical.forall_intro_2 prf
+
+let array_group3_concat_unique_strong_strong_prefix
+  #b (a1 a2: array_group3 b)
+: Lemma
+  (requires (
+    array_group3_concat_unique_strong a1 a2 /\
+    array_group3_strong_prefix a2
+  ))
+  (ensures (
+    array_group3_strong_prefix (array_group3_concat a1 a2)
+  ))
+= array_group3_concat_unique_strong'_strong_prefix a1 a2
+
+let array_group3_concat_unique_strong_concat
+  #b (a1 a2 a3: array_group3 b)
+: Lemma
+  (requires (
+    array_group3_concat_unique_strong a1 a2
+  ))
+  (ensures (
+    array_group3_concat_unique_strong a1 (array_group3_concat a2 a3)
+  ))
+= ()
+
 let array_group3_choice #b (a1 a3: array_group3 b) : array_group3 b =
   fun l -> match a1 l with
     | None -> a3 l
     | Some l3 -> Some l3
 
-let rec array_group3_zero_or_more' #b (a: array_group3 b) (l: list Cbor.raw_data_item { opt_precedes l b }) : Ghost (option (list Cbor.raw_data_item))
+let array_group3_concat_unique_strong_choice_right #b (a1 a2 a3: array_group3 b) : Lemma
+  (requires (
+    array_group3_concat_unique_strong a1 a2 /\
+    array_group3_concat_unique_strong a1 a3
+  ))
+  (ensures (
+    array_group3_concat_unique_strong a1 (array_group3_choice a2 a3)
+  ))
+= ()
+
+let array_group3_disjoint #b (a1 a2: array_group3 b) : Tot prop
+= (forall (l: list Cbor.raw_data_item { opt_precedes_list l b }) . ~ (Some? (a1 l) /\ Some? (a2 l)))
+
+let array_group3_concat_unique_strong_choice_left #b (a1 a2 a3: array_group3 b) : Lemma
+  (requires (
+    array_group3_concat_unique_strong a1 a3 /\
+    array_group3_concat_unique_strong a2 a3 /\
+    array_group3_disjoint a1 a2
+  ))
+  (ensures (
+    array_group3_concat_unique_strong (array_group3_choice a1 a2) a3
+  ))
+= ()
+
+let array_group3_disjoint_sym #b (a1 a2: array_group3 b) : Lemma
+  (array_group3_disjoint a1 a2 <==> array_group3_disjoint a2 a1)
+= ()
+
+let array_group3_disjoint_choice #b (a1 a2 a3: array_group3 b) : Lemma
+  (requires (
+    array_group3_disjoint a1 a2 /\
+    array_group3_disjoint a1 a3
+  ))
+  (ensures (
+    array_group3_disjoint a1 (array_group3_choice a2 a3)
+  ))
+= ()
+
+let array_group3_disjoint_concat #b (a1 a2 a3: array_group3 b) : Lemma
+  (requires (array_group3_disjoint a1 a2))
+  (ensures (array_group3_disjoint a1 (array_group3_concat a2 a3)))
+= ()
+
+let rec array_group3_zero_or_more' #b (a: array_group3 b) (l: list Cbor.raw_data_item { opt_precedes_list l b }) : Ghost (option (list Cbor.raw_data_item & list Cbor.raw_data_item))
   (requires True)
-  (ensures (fun l' -> match l' with None -> True | Some l' -> opt_precedes l' b))
+  (ensures (fun l' -> match l' with None -> True | Some (l1, l2) -> l == l1 `List.Tot.append` l2))
   (decreases (List.Tot.length l))
 =
   match a l with
-  | None -> Some l
-  | Some l' ->
-    if List.Tot.length l' >= List.Tot.length l
-    then Some l
-    else array_group3_zero_or_more' a l'
+  | None -> Some ([], l)
+  | Some (l1, l2) ->
+    List.Tot.append_length l1 l2;
+    if Nil? l1
+    then Some (l1, l2)
+    else
+      begin match array_group3_zero_or_more' a l2 with
+      | None -> None
+      | Some (l2', l3) -> List.Tot.append_assoc l1 l2' l3; Some (List.Tot.append l1 l2', l3)
+      end
 
 let array_group3_zero_or_more #b : array_group3 b -> array_group3 b = array_group3_zero_or_more'
+
+let rec array_group3_zero_or_more_some
+  #b
+  (a: array_group3 b)
+  (l: list Cbor.raw_data_item { opt_precedes_list l b })
+: Lemma
+  (ensures (Some? (array_group3_zero_or_more a l)))
+  (decreases List.Tot.length l)
+  [SMTPat (array_group3_zero_or_more a l)]
+= match a l with
+  | None -> ()
+  | Some (l1, l2) ->
+    List.Tot.append_length l1 l2;
+    if Nil? l1
+    then ()
+    else array_group3_zero_or_more_some a l2
+
+let array_group3_concat_unique_strong_concat_zero_or_more_right
+  #b (a1 a2 a3: array_group3 b)
+: Lemma
+  (requires (
+    array_group3_concat_unique_strong a1 a2 /\
+    array_group3_concat_unique_strong a1 a3
+  ))
+  (ensures (
+    array_group3_concat_unique_strong a1 (array_group3_concat (array_group3_zero_or_more a2) a3)
+  ))
+= ()
+
+let array_group3_concat_unique_strong_zero_or_more_right
+  #b (a1 a2: array_group3 b)
+: Lemma
+  (ensures (
+    array_group3_concat_unique_strong a1 (array_group3_zero_or_more a2) <==> array_group3_strong_prefix a1
+  ))
+= ()
+
+let array_group3_concat_unique_strong'_zero_or_more_left
+  #b (a1 a2: array_group3 b)
+: Lemma
+  (requires (
+    array_group3_disjoint a1 a2 /\
+    array_group3_concat_unique_strong' a1 a1 /\
+    array_group3_concat_unique_strong' a1 a2
+  ))
+  (ensures (
+    array_group3_concat_unique_strong' (array_group3_zero_or_more a1) a2
+  ))
+= let _ : squash (array_group3_disjoint a1 a2) = () in
+  let rec prf
+    (l1 l2: (l: list Cbor.raw_data_item { opt_precedes_list l b }))
+  : Lemma
+    (ensures (
+      Some? (a2 l2) ==> (array_group3_zero_or_more a1 l1 == Some (l1, []) <==> array_group3_zero_or_more a1 (l1 `List.Tot.append` l2) == Some (l1, l2))
+    ))
+    (decreases (List.Tot.length l1))
+  = if Some? (a2 l2)
+    then begin
+      if FStar.StrongExcludedMiddle.strong_excluded_middle (array_group3_zero_or_more a1 l1 == Some (l1, []))
+      then
+        match a1 l1 with
+        | None -> ()
+        | Some (l1l, l1r) ->
+          if Nil? l1l
+          then ()
+          else begin
+            List.Tot.append_length l1l l1r;
+            List.Tot.append_assoc l1l l1r l2;
+            let Some (l1rl, l1rr) = array_group3_zero_or_more a1 l1r in
+            assert (Nil? l1rr);
+            List.Tot.append_l_nil l1rl;
+            prf l1r l2
+          end
+      else if FStar.StrongExcludedMiddle.strong_excluded_middle (array_group3_zero_or_more a1 (l1 `List.Tot.append` l2) == Some (l1, l2))
+      then begin
+        match a1 (l1 `List.Tot.append` l2) with
+        | None -> ()
+        | Some (l12l, l12r) ->
+          let Some (l12rl, l12rr) = array_group3_zero_or_more a1 l12r in
+          assert (l12rr == l2);
+          List.Tot.append_assoc l12l l12rl l2;
+          List.Tot.append_length l12rl l12rr;
+          List.Tot.append_length l12l l12r;
+          List.Tot.append_length l1 l2;
+          if Nil? l12l
+          then ()
+          else begin
+            prf l12rl l2
+          end
+      end
+    end
+  in
+  Classical.forall_intro_2 prf
+
+let array_group3_concat_unique_strong_zero_or_more_left
+  #b (a1 a2: array_group3 b)
+: Lemma
+  (requires (
+    array_group3_disjoint a1 a2 /\
+    array_group3_concat_unique_strong a1 a1 /\
+    array_group3_concat_unique_strong a1 a2
+  ))
+  (ensures (
+    array_group3_concat_unique_strong (array_group3_zero_or_more a1) a2
+  ))
+= array_group3_concat_unique_strong'_zero_or_more_left a1 a2
+
+let array_group3_concat_unique_weak
+  #b (a1 a3: array_group3 b)
+: Tot prop
+= (forall (l: (l: list Cbor.raw_data_item { opt_precedes_list l b })) .
+    array_group3_concat a1 a3 l == Some (l, []) ==> (
+      (exists (l1 l2: list Cbor.raw_data_item) .
+        a1 l == Some (l1, l2) /\
+        a1 l1 == Some (l1, []) /\
+        a3 l2 == Some (l2, [])
+  ))) /\
+  (forall (l1 l2: (l: list Cbor.raw_data_item { opt_precedes_list l b })) .
+    (a1 l1 == Some (l1, []) /\ a3 l2 == Some (l2, [])) ==>
+    a1 (l1 `List.Tot.append` l2) == Some (l1, l2)
+  )
+
+let list_append_l_nil
+  (#t: Type)
+  (l: list t)
+: Lemma
+  (l `List.Tot.append` [] == l)
+  [SMTPat (l `List.Tot.append` [])]
+= List.Tot.append_l_nil l
+
+let array_group3_concat_unique_strong_implies_weak
+  #b (a1 a3: array_group3 b)
+: Lemma
+  (array_group3_concat_unique_strong a1 a3 ==> array_group3_concat_unique_weak a1 a3)
+= ()
+
+#push-options "--z3rlimit 16"
+#restart-solver
+
+let array_group3_concat_unique_weak_concat_zero_or_more_right
+  #b (a1 a2 a3: array_group3 b)
+: Lemma
+  (requires (
+    array_group3_concat_unique_strong a1 a2 /\
+    array_group3_concat_unique_weak a1 a3
+  ))
+  (ensures (
+    array_group3_concat_unique_weak a1 (array_group3_concat (array_group3_zero_or_more a2) a3)
+  ))
+= ()
+
+let array_group3_concat_unique_weak_zero_or_more_left'
+  #b (a1 a2: array_group3 b)
+: Lemma
+  (requires (
+    array_group3_disjoint a1 a2 /\
+    array_group3_concat_unique_strong' a1 a1 /\
+    array_group3_concat_unique_weak a1 a2
+  ))
+  (ensures (
+    array_group3_concat_unique_weak (array_group3_zero_or_more a1) a2
+  ))
+= let a10 = a1 in
+  let a1 = array_group3_zero_or_more a10 in
+  let a3 = a2 in
+  let rec prf2
+    (l1 l2: (l: list Cbor.raw_data_item { opt_precedes_list l b }))
+  : Lemma
+    (ensures ((a1 l1 == Some (l1, []) /\ a3 l2 == Some (l2, [])) ==>
+    a1 (l1 `List.Tot.append` l2) == Some (l1, l2)))
+    (decreases (List.Tot.length l1))
+  = if FStar.StrongExcludedMiddle.strong_excluded_middle (a1 l1 == Some (l1, []) /\ a3 l2 == Some (l2, []))
+    then match a10 l1 with
+    | None -> ()
+    | Some (l1l, l1r) ->
+      if Nil? l1l
+      then ()
+      else begin
+        List.Tot.append_length l1l l1r;
+        List.Tot.append_assoc l1l l1r l2;
+        prf2 l1r l2
+      end
+  in
+  let rec prf1
+    (l: (l: list Cbor.raw_data_item { opt_precedes_list l b }))
+  : Lemma
+    (ensures (array_group3_concat a1 a3 l == Some (l, []) ==> (
+      (exists (l1 l2: list Cbor.raw_data_item) .
+        a1 l == Some (l1, l2) /\
+        a1 l1 == Some (l1, []) /\
+        a3 l2 == Some (l2, [])
+    ))))
+    (decreases (List.Tot.length l))
+  = if FStar.StrongExcludedMiddle.strong_excluded_middle (array_group3_concat a1 a3 l == Some (l, []))
+    then match a10 l with
+    | None -> ()
+    | Some (l1l, l1r) ->
+      if Nil? l1l
+      then ()
+      else begin
+        List.Tot.append_length l1l l1r;
+        prf1 l1r;
+        let Some (l2l, l2r) = a1 l1r in
+        List.Tot.append_assoc l1l l2l l2r
+      end
+  in
+  Classical.forall_intro prf1;
+  Classical.forall_intro_2 prf2
+
+#pop-options
+
+let array_group3_concat_unique_weak_zero_or_more_left
+  #b (a1 a2: array_group3 b)
+: Lemma
+  (requires (
+    array_group3_disjoint a1 a2 /\
+    array_group3_concat_unique_strong a1 a1 /\
+    array_group3_concat_unique_weak a1 a2
+  ))
+  (ensures (
+    array_group3_concat_unique_weak (array_group3_zero_or_more a1) a2
+  ))
+= array_group3_concat_unique_weak_zero_or_more_left' a1 a2
+
+let array_group3_concat_unique_weak_zero_or_more_right
+  #b (a1 a2: array_group3 b)
+: Lemma
+  (requires (
+    array_group3_concat_unique_strong a1 a2
+  ))
+  (ensures (
+    array_group3_concat_unique_weak a1 (array_group3_zero_or_more a2)
+  ))
+= ()
+
+#push-options "--z3rlimit 16"
+#restart-solver
+
+let array_group3_concat_unique_weak_zero_or_more'
+  #b (a1 a2: array_group3 b)
+: Lemma
+  (requires (
+    array_group3_concat_unique_strong' a1 a1 /\
+    array_group3_concat_unique_strong' a1 a2 /\
+    array_group3_disjoint a1 a2
+  ))
+  (ensures (
+    array_group3_concat_unique_weak (array_group3_zero_or_more a1) (array_group3_zero_or_more a2)
+  ))
+= let a10 = a1 in
+  let a1 = array_group3_zero_or_more a10 in
+  let a3 = array_group3_zero_or_more a2 in
+  let rec prf2
+    (l1 l2: (l: list Cbor.raw_data_item { opt_precedes_list l b }))
+  : Lemma
+    (ensures ((a1 l1 == Some (l1, []) /\ a3 l2 == Some (l2, [])) ==>
+    a1 (l1 `List.Tot.append` l2) == Some (l1, l2)))
+    (decreases (List.Tot.length l1))
+  = if FStar.StrongExcludedMiddle.strong_excluded_middle (a1 l1 == Some (l1, []) /\ a3 l2 == Some (l2, []))
+    then match a10 l1 with
+    | None -> ()
+    | Some (l1l, l1r) ->
+      if Nil? l1l
+      then ()
+      else begin
+        List.Tot.append_length l1l l1r;
+        List.Tot.append_assoc l1l l1r l2;
+        prf2 l1r l2
+      end
+  in
+  let rec prf1
+    (l: (l: list Cbor.raw_data_item { opt_precedes_list l b }))
+  : Lemma
+    (ensures (array_group3_concat a1 a3 l == Some (l, []) ==> (
+      (exists (l1 l2: list Cbor.raw_data_item) .
+        a1 l == Some (l1, l2) /\
+        a1 l1 == Some (l1, []) /\
+        a3 l2 == Some (l2, [])
+    ))))
+    (decreases (List.Tot.length l))
+  = if FStar.StrongExcludedMiddle.strong_excluded_middle (array_group3_concat a1 a3 l == Some (l, []))
+    then match a10 l with
+    | None -> ()
+    | Some (l1l, l1r) ->
+      if Nil? l1l
+      then ()
+      else begin
+        List.Tot.append_length l1l l1r;
+        prf1 l1r;
+        let Some (l2l, l2r) = a1 l1r in
+        List.Tot.append_assoc l1l l2l l2r
+      end
+  in
+  Classical.forall_intro prf1;
+  Classical.forall_intro_2 prf2
+
+#pop-options
+
+let array_group3_concat_unique_weak_zero_or_more
+  #b (a1 a2: array_group3 b)
+: Lemma
+  (requires (
+    array_group3_concat_unique_strong a1 a1 /\
+    array_group3_concat_unique_strong a1 a2 /\
+    array_group3_disjoint a1 a2
+  ))
+  (ensures (
+    array_group3_concat_unique_weak (array_group3_zero_or_more a1) (array_group3_zero_or_more a2)
+  ))
+= array_group3_concat_unique_weak_zero_or_more' a1 a2
+
+let array_group3_concat_unique_weak_choice_right #b (a1 a2 a3: array_group3 b) : Lemma
+  (requires (
+    array_group3_concat_unique_weak a1 a2 /\
+    array_group3_concat_unique_weak a1 a3
+  ))
+  (ensures (
+    array_group3_concat_unique_weak a1 (array_group3_choice a2 a3)
+  ))
+= ()
+
+let array_group3_concat_unique_weak_choice_left #b (a1 a2 a3: array_group3 b) : Lemma
+  (requires (
+    array_group3_concat_unique_weak a1 a3 /\
+    array_group3_concat_unique_weak a2 a3 /\
+    array_group3_disjoint a1 a2
+  ))
+  (ensures (
+    array_group3_concat_unique_weak (array_group3_choice a1 a2) a3
+  ))
+= ()
 
 let array_group3_one_or_more #b (a: array_group3 b) : array_group3 b =
   a `array_group3_concat` array_group3_zero_or_more a
@@ -289,7 +914,7 @@ let array_group3_zero_or_one #b (a: array_group3 b) : Tot (array_group3 b) =
 let array_group3_item (#b: option Cbor.raw_data_item) (t: bounded_typ_gen b) : array_group3 b = fun l ->
   match l with
   | [] -> None
-  | a :: q -> if t a then Some q else None
+  | a :: q -> if t a then Some ([a], q) else None
 
 let array_group3_item_equiv
   #b
@@ -300,10 +925,10 @@ let array_group3_item_equiv
 = ()
 
 let match_array_group3 (#b: option Cbor.raw_data_item) (a: array_group3 b)
-  (l: list Cbor.raw_data_item {opt_precedes l b})
+  (l: list Cbor.raw_data_item {opt_precedes_list l b})
 : GTot bool
 = match a l with
-  | Some l' -> Nil? l'
+  | Some (_, l') -> Nil? l'
   | _ -> false
 
 let t_array3 (#b: option Cbor.raw_data_item) (a: array_group3 b) : bounded_typ_gen b = fun x ->
@@ -341,8 +966,6 @@ let rec t_array3_rec
 [@@erasable]
 noeq
 type map_group_entry (b: option Cbor.raw_data_item) = | MapGroupEntry: (fst: bounded_typ_gen b) -> (snd: bounded_typ_gen b) -> map_group_entry b
-
-module Pull = FStar.Ghost.Pull
 
 noextract
 let opt_map_entry_bounded'
